x64 port of the x86 CBC code - Introduce Xor64 instruction - Change x64 definition of 'while' and 'if' to use 64-bit conditionals

src/lib/util/types.s.dfy
@@ -55,4 +55,13 @@ lemma {:axiom} lemma_BitsToWordToBits(b:bv32)
 lemma {:axiom} lemma_WordToBitsToWord(w:uint32)
     ensures BitsToWord(WordToBits(w)) == w;
 
+function method {:opaque} BitsToWord64(b:bv64) : uint64 { b as uint64 }
+function method {:opaque} WordToBits64(w:uint64) : bv64 { w as bv64 }
+
+lemma {:axiom} lemma_BitsToWordToBits64(b:bv64)
+    ensures WordToBits64(BitsToWord64(b)) == b;
+
+lemma {:axiom} lemma_WordToBitsToWord64(w:uint64)
+    ensures BitsToWord64(WordToBits64(w)) == w;
+
 } // end module types_s
