src/arch/x64/printMasm.s.dfy
@@ -174,6 +174,7 @@ method printIns(ins:ins)
         case AddCarry(dst, src) => print ("  add "); printOprnd(dst); print(", "); printOprnd(src); print("\n");
         case BSwap32(dst)    => print ("  bswap "); printOprnd(dst); print("\n");
         case Xor32(dst, src) => print ("  xor "); printOprnd(dst); print(", "); printOprnd(src); print("\n");
+        case Xor64(dst, src) => print ("  xor "); printOprnd(dst); print(", "); printOprnd(src); print("\n");
         case And32(dst, src) => print ("  and "); printOprnd(dst); print(", "); printOprnd(src); print("\n");
         case Not32(dst)      => print ("  not "); printOprnd(dst); print("\n");
         case GetCf(dst)      => print ("  setc "); printSmallOprnd(dst); print("\n");
